thys/HRB-Slicing/StaticInter/FundamentalProperty.thy
@@ -2061,7 +2061,7 @@ subsection {* @{text "n\<^isub>c,f \<turnstile> (ms,s) =as\<Rightarrow>* (ms',s'
 
 
 inductive trans_observable_moves :: 
-  "'node SDG_node \<Rightarrow> ('edge \<Rightarrow> ('var,'val,'ret) edge_kind) \<Rightarrow> 'node list \<Rightarrow> 
+  "'node SDG_node \<Rightarrow> ('edge \<Rightarrow> ('var,'val,'ret,'pname) edge_kind) \<Rightarrow> 'node list \<Rightarrow> 
    (('var \<rightharpoonup> 'val) \<times> 'ret) list \<Rightarrow> 'edge list \<Rightarrow> 'node list \<Rightarrow> 
   (('var \<rightharpoonup> 'val) \<times> 'ret) list \<Rightarrow> bool"
 ("_,_ \<turnstile> '(_,_') =_\<Rightarrow>* '(_,_')" [51,50,0,0,50,0,0] 51) 
@@ -3452,10 +3452,11 @@ locale SemanticsProperty = SDG sourcenode targetnode kind valid_edge Entry
   CFG_semantics_wf sourcenode targetnode kind valid_edge Entry 
     get_proc get_return_edges procs Main sem identifies
   for sourcenode :: "'edge \<Rightarrow> 'node" and targetnode :: "'edge \<Rightarrow> 'node"
-  and kind :: "'edge \<Rightarrow> ('var,'val,'ret) edge_kind" and valid_edge :: "'edge \<Rightarrow> bool"
-  and Entry :: "'node" ("'('_Entry'_')")  and get_proc :: "'node \<Rightarrow> pname"
+  and kind :: "'edge \<Rightarrow> ('var,'val,'ret,'pname) edge_kind" 
+  and valid_edge :: "'edge \<Rightarrow> bool"
+  and Entry :: "'node" ("'('_Entry'_')")  and get_proc :: "'node \<Rightarrow> 'pname"
   and get_return_edges :: "'edge \<Rightarrow> 'edge set"
-  and procs :: "(pname \<times> 'var list \<times> 'var list) list" and Main :: "pname"
+  and procs :: "('pname \<times> 'var list \<times> 'var list) list" and Main :: "'pname"
   and Exit::"'node"  ("'('_Exit'_')") 
   and Def :: "'node \<Rightarrow> 'var set" and Use :: "'node \<Rightarrow> 'var set"
   and ParamDefs :: "'node \<Rightarrow> 'var list" and ParamUses :: "'node \<Rightarrow> 'var set list"
