thys/HRB-Slicing/StaticInter/Postdomination.thy
@@ -8,10 +8,11 @@ text {* For static interprocedural slicing, we only consider standard control
 locale Postdomination = CFGExit sourcenode targetnode kind valid_edge Entry 
     get_proc get_return_edges procs Main Exit
   for sourcenode :: "'edge \<Rightarrow> 'node" and targetnode :: "'edge \<Rightarrow> 'node"
-  and kind :: "'edge \<Rightarrow> ('var,'val,'ret) edge_kind" and valid_edge :: "'edge \<Rightarrow> bool"
-  and Entry :: "'node" ("'('_Entry'_')")  and get_proc :: "'node \<Rightarrow> pname"
+  and kind :: "'edge \<Rightarrow> ('var,'val,'ret,'pname) edge_kind" 
+  and valid_edge :: "'edge \<Rightarrow> bool"
+  and Entry :: "'node" ("'('_Entry'_')")  and get_proc :: "'node \<Rightarrow> 'pname"
   and get_return_edges :: "'edge \<Rightarrow> 'edge set"
-  and procs :: "(pname \<times> 'var list \<times> 'var list) list" and Main :: "pname"
+  and procs :: "('pname \<times> 'var list \<times> 'var list) list" and Main :: "'pname"
   and Exit::"'node"  ("'('_Exit'_')") +
   assumes Entry_path:"valid_node n \<Longrightarrow> \<exists>as. (_Entry_) -as\<rightarrow>\<^isub>\<surd>* n"
   and Exit_path:"valid_node n \<Longrightarrow> \<exists>as. n -as\<rightarrow>\<^isub>\<surd>* (_Exit_)"
