thys/HRB-Slicing/StaticInter/WeakSimulation.thy
@@ -208,7 +208,7 @@ qed
 subsection {* Silent moves *}
 
 inductive silent_move :: 
-  "'node SDG_node \<Rightarrow> ('edge \<Rightarrow> ('var,'val,'ret) edge_kind) \<Rightarrow> 'node list \<Rightarrow> 
+  "'node SDG_node \<Rightarrow> ('edge \<Rightarrow> ('var,'val,'ret,'pname) edge_kind) \<Rightarrow> 'node list \<Rightarrow> 
   (('var \<rightharpoonup> 'val) \<times> 'ret) list \<Rightarrow> 'edge \<Rightarrow> 'node list \<Rightarrow> (('var \<rightharpoonup> 'val) \<times> 'ret) list \<Rightarrow> bool"
 ("_,_ \<turnstile> '(_,_') -_\<rightarrow>\<^isub>\<tau> '(_,_')" [51,50,0,0,50,0,0] 51) 
 
@@ -600,7 +600,7 @@ qed
 
 
 inductive silent_moves :: 
-  "'node SDG_node \<Rightarrow> ('edge \<Rightarrow> ('var,'val,'ret) edge_kind) \<Rightarrow> 'node list \<Rightarrow> 
+  "'node SDG_node \<Rightarrow> ('edge \<Rightarrow> ('var,'val,'ret,'pname) edge_kind) \<Rightarrow> 'node list \<Rightarrow> 
   (('var \<rightharpoonup> 'val) \<times> 'ret) list \<Rightarrow> 'edge list \<Rightarrow> 'node list \<Rightarrow> (('var \<rightharpoonup> 'val) \<times> 'ret) list \<Rightarrow> bool"
 ("_,_ \<turnstile> '(_,_') =_\<Rightarrow>\<^isub>\<tau> '(_,_')" [51,50,0,0,50,0,0] 51)
 
@@ -1163,7 +1163,7 @@ subsection {* Observable moves *}
 
 
 inductive observable_move ::
-  "'node SDG_node \<Rightarrow> ('edge \<Rightarrow> ('var,'val,'ret) edge_kind) \<Rightarrow> 'node list \<Rightarrow> 
+  "'node SDG_node \<Rightarrow> ('edge \<Rightarrow> ('var,'val,'ret,'pname) edge_kind) \<Rightarrow> 'node list \<Rightarrow> 
    (('var \<rightharpoonup> 'val) \<times> 'ret) list \<Rightarrow> 'edge \<Rightarrow> 'node list \<Rightarrow> (('var \<rightharpoonup> 'val) \<times> 'ret) list \<Rightarrow> bool"
 ("_,_ \<turnstile> '(_,_') -_\<rightarrow> '(_,_')" [51,50,0,0,50,0,0] 51) 
  
@@ -1192,7 +1192,7 @@ inductive observable_move ::
 
 
 inductive observable_moves :: 
-  "'node SDG_node \<Rightarrow> ('edge \<Rightarrow> ('var,'val,'ret) edge_kind) \<Rightarrow> 'node list \<Rightarrow> 
+  "'node SDG_node \<Rightarrow> ('edge \<Rightarrow> ('var,'val,'ret,'pname) edge_kind) \<Rightarrow> 'node list \<Rightarrow> 
    (('var \<rightharpoonup> 'val) \<times> 'ret) list \<Rightarrow> 'edge list \<Rightarrow> 'node list \<Rightarrow> (('var \<rightharpoonup> 'val) \<times> 'ret) list \<Rightarrow> bool"
 ("_,_ \<turnstile> '(_,_') =_\<Rightarrow> '(_,_')" [51,50,0,0,50,0,0] 51) 
 
